small fix

theories/typing/bool.v
@@ -3,25 +3,23 @@ From lrust.typing Require Import programs.
 
 Set Default Proof Using "Type".
 
-Implicit Type b: boolₛ.
-
 Section bool.
   Context `{!typeG Σ}.
 
   Program Definition bool_ty: type boolₛ :=
-    {| pt_size := 1;  pt_own b _ vl := ⌜vl = [ #b]⌝; |}%I.
+    {| pt_size := 1;  pt_own (b: boolₛ) _ vl := ⌜vl = [ #b]⌝; |}%I.
   Next Obligation. move=> *. by iIntros (->). Qed.
 
   Global Instance bool_send: Send bool_ty. Proof. done. Qed.
 
-  Lemma type_bool_instr b : typed_val #b bool_ty (λ post, post b).
+  Lemma type_bool_instr (b: bool) : typed_val #b bool_ty (λ post, post b).
   Proof.
     iIntros (?????) "_ _ _ _ _ $$ _ Obs". iMod persist_time_rcpt_0 as "⧖".
     iApply wp_value. iExists -[const b]. iFrame "Obs". iSplit; [|done].
     rewrite tctx_hasty_val'; [|done]. iExists 0%nat. iFrame "⧖". by iExists b.
   Qed.
 
-  Lemma type_bool {𝔄l} b E L C (T: _ 𝔄l) x e tr:
+  Lemma type_bool {𝔄l} (b: bool) (T: _ 𝔄l) x e tr E L C :
     Closed (x :b: []) e →
     (∀v: val, typed_body E L C (v ◁ bool_ty +:: T) (subst' x v e) tr) -∗
     typed_body E L C T (let: x := #b in e) (λ al, tr (b -:: al)).
@@ -33,9 +31,9 @@ Section bool.
     typed_body E L C T (if: p then e1 else e2)
       (tr (λ '(b -:: vl), if b then pre1 vl else pre2 vl)).
   Proof.
-    iIntros (?) "e1 e2". iApply typed_body_tctx_incl; [done|]. iIntros (?[??]).
-    iIntros "#LFT #TIME #PROPH #UNIQ #E Na L C [p T] Obs". wp_bind p.
-    iApply (wp_hasty with "p"). iIntros (?? _) "_".
+    iIntros (?) "e1 e2". iApply typed_body_tctx_incl; [done|]=>/=.
+    iIntros (?[??]) "/= #LFT #TIME #PROPH #UNIQ #E Na L C [p T] Obs".
+    wp_bind p. iApply (wp_hasty with "p"). iIntros (?? _) "_".
     iDestruct 1 as ([|]->) "%Eq"; move: Eq=> [=->]; wp_case.
     - by iApply ("e1" with "LFT TIME PROPH UNIQ E Na L C T").
     - by iApply ("e2" with "LFT TIME PROPH UNIQ E Na L C T").
